compiler/backend/stack_removeScript.sml
@@ -93,7 +93,7 @@ val comp_def = Define `
     | StackGetSize r => Seq (Inst (Arith (Binop Sub r k (Reg (k+1)))))
                             (right_shift_inst r (word_shift (:'a)))
     | StackSetSize r => Seq (Inst (Arith (Binop Add k (k+1) (Reg r))))
-                            (left_shift_inst r (word_shift (:'a)))
+                            (left_shift_inst k (word_shift (:'a)))
     | BitmapLoad r v =>
         list_Seq [Inst (Mem Load r (Addr (k+1) (store_offset BitmapBase)));
                   add_inst r v;
